forcing/GRTT.v
@@ -1,0 +1,66 @@
+(* Formalisation of Guarded Recursive Types using the cbn forcing translation in Template Coq
+   with the ordered set of natural numbers as forcing conditions *)
+
+Require Import String.
+Require Import Forcing.TemplateForcing.
+
+Open Scope string.
+
+(** Yoneda embedding  *)
+Definition nat_obj := nat.
+Definition nat_hom := (fun (P Q : nat_obj) => forall R, Q <= R -> P <= R).
+Definition id_nat_hom (P : nat_obj) := (fun (R : nat_obj) (k : P <= R) => k).
+Definition nat_comp (P Q R : nat_obj) (g : nat_hom Q R) (f : nat_hom P Q)
+  := (fun (S : nat_obj) (k : R <= S) => f S (g S k)).
+
+Notation "P ≤ Q" := (nat_hom P Q) (at level 70).
+Notation "#" := id_nat_hom.
+Notation "f ∘ g" := (fun (R : nat_obj) (k : _ <= R) => f R (g R k)) (at level 40).
+
+(* Now, laws hold definitionally *)
+Lemma nat_cat_left_id P R (g : R ≤ P)  : (id_nat_hom R) ∘ g = g.
+Proof. reflexivity. Qed.
+
+Lemma nat_cat_right_id P R (f : P ≤ R)  : f ∘ (id_nat_hom R) = f.
+Proof. reflexivity. Qed.
+
+Lemma nat_cat_assoc P Q R S (f : P ≤ Q) (g : Q ≤ R) (h : R ≤ S):
+  f ∘ (g ∘ h) = (f ∘ g) ∘ h.
+Proof. reflexivity. Qed.
+
+Definition nat_cat : category :=
+  makeCat "nat_obj" "nat_hom" "id_nat_hom" "nat_comp".
+
+(** Copied from the template coq demo *)
+
+(** This is just printing **)
+Test Quote (fun x : nat => x * x).
+
+Test Quote (fun (f : nat -> nat) (x : nat) => f x).
+
+Test Quote (let x := 2 in x).
+
+Test Quote (let x := 2 in
+            match x with
+              | 0 => 0
+              | S n => n
+            end).
+
+(** Build a definition **)
+Definition d : Ast.term.
+  let t := constr:(fun x : nat => x) in
+  let k x := refine x in
+  quote_term t k.
+Defined.
+
+Print d.
+
+(** Another way **)
+Quote Definition d' := (fun x : nat => x).
+
+(** To quote existing definitions **)
+Definition id_nat : nat -> nat := fun x => x.
+
+Quote Definition d'' := Eval compute in id_nat.
+
+Print d''.
